{
 "metadata": {
  "name": "",
  "signature": "sha256:6dd36e27bb2bd8e23d3aad8539e9b7cfde2a2b6c534de690b5269ce67f7dae0f"
 },
 "nbformat": 3,
 "nbformat_minor": 0,
 "worksheets": [
  {
   "cells": [
    {
     "cell_type": "markdown",
     "metadata": {},
     "source": [
      "## Definitions\n",
      "\\begin{align*}\n",
      "h(x)&=f(x)*g(x)=\\int_{-\\pi}^{\\pi}f(x-y)g(y)dy\\\\\n",
      "f(x)&=\\sum_{k=-\\infty}^\\infty c_k\\exp(ikx)\\\\\n",
      "c_k&=\\int_{-\\pi}^{\\pi}f(x)\\exp(-ikx)dx\\\\\n",
      "g(x)&=\\sum_{k=-\\infty}^\\infty d_k\\exp(ikx)\\\\\n",
      "d_k&=\\int_{-\\pi}^{\\pi}g(x)\\exp(-ikx)dx\\\\\n",
      "h(x)&=\\sum_{k=-\\infty}^\\infty e_k\\exp(ikx)\n",
      "\\end{align*}\n",
      "\n",
      "## Part (a)\n",
      "\n",
      "Find $e_k$ the complex coefficients for $h(x)$.\n",
      "\n",
      "\\begin{align*}\n",
      "h(x)&=\\int_{-\\pi}^{\\pi}f(x-y)g(y)dy\\\\\n",
      "&=\\int_{-\\pi}^{\\pi}\\sum_{k=-\\infty}^\\infty c_k\\exp(ik(x-y))\\sum_{j=-\\infty}^\\infty d_j\\exp(ijy)dy\\\\\n",
      "\\end{align*}\n",
      "\n",
      "Consider a single multiple from the polynomial multiplication, $k=n,j=m\\in\\Z$:\n",
      "\n",
      "\\begin{align*}\n",
      "I&=\\int_{-\\pi}^{\\pi} c_m\\exp(im(x-y))d_n\\exp(iny)dy\\\\\n",
      "&=c_md_n\\exp(imx)\\int_{-\\pi}^{\\pi} \\exp(iny-imy)dy\\\\\n",
      "&=c_md_n\\exp(imx)\\int_{-\\pi}^{\\pi} \\exp(iy(n-m))dy\n",
      "\\end{align*}\n",
      "\n",
      "\\pagebreak\n",
      "\n",
      "Case 1: $n=m$\n",
      "\\begin{align*}\n",
      "I&=c_md_n\\exp(imx)\\int_{-\\pi}^{\\pi} dy\\\\\n",
      "&=2\\pi c_md_n\\exp(imx)\n",
      "\\end{align*}\n",
      "\n",
      "Case 2: $n\\neq m$\n",
      "\n",
      "\\begin{align*}\n",
      "I&=c_md_n\\exp(imx)\\int_{-\\pi}^{\\pi} dy\\\\\n",
      "&=c_md_n\\exp(imx)\\int_{-\\pi}^{\\pi} \\exp(iy(n-m))dy\\\\\n",
      "&=\\frac{c_md_n\\exp(imx)}{i(n-m)}\\exp(iy(n-m))\\bigg|_{-\\pi}^{\\pi}\\\\\n",
      "&=\\frac{c_md_n\\exp(imx)}{i(n-m)}\\bigP{\\exp(i\\pi(n-m))-\\exp(-i\\pi(n-m))}=0\\\\\n",
      "\\end{align*}\n",
      "\n",
      "Therefore, \n",
      "\n",
      "\n",
      "\\begin{align*}\n",
      "h(x)&=\\int_{-\\pi}^{\\pi}\\sum_{k=-\\infty}^\\infty c_kd_k\\exp(ik(x-y)+iky)dy\\\\\n",
      "&=\\sum_{k=-\\infty}^\\infty c_kd_k\\exp(ikx)\\int_{-\\pi}^{\\pi}dy\\\\\n",
      "&=2\\pi\\sum_{k=-\\infty}^\\infty c_kd_k\\exp(ikx)\n",
      "\\end{align*}\n",
      "\n",
      "And, \n",
      "\n",
      "$$e_k=2\\pi c_kd_k$$\n",
      "\n",
      "## Part (b)\n",
      "\n",
      "For $\\cos 3x$, $a_3=1$ with $b_k=0$ and $a_{k\\neq3}=0$. Therefore, $c_3=\\frac{1}{2}$ and $c_{-3}=\\frac{1}{2}$ with all $c_{k\\neq 3,-3}=0$.\n",
      "\n",
      "For $\\sin 2x$, $b_2=1$ with $a_k=0$ and $b_{k\\neq2}=0$. Therefore, $d_2=\\frac{-i}{2}$ and $d_{-2}=\\frac{i}{2}$ with all $d_{k\\neq 2,-2}=0$.\n",
      "\n",
      "All $e_{k\\neq-3,-2,2,3}$ will trivially be 0. \n",
      "\n",
      "\\begin{align*}\n",
      "e_{-3}&=\\frac{1}{2}\\cdot0=0\\\\\n",
      "e_{-2}&=0\\cdot\\frac{i}{2}=0\\\\\n",
      "e_2&=0\\cdot\\frac{-i}{2}=0\\\\\n",
      "e_3&=\\frac{1}{2}\\cdot0=0\n",
      "\\end{align*}"
     ]
    },
    {
     "cell_type": "markdown",
     "metadata": {},
     "source": [
      "# Derivation of the Momentum Operator\n",
      "\n",
      "\\begin{align*}\n",
      "\\left\\langle \\hat{p}_x \\right\\rangle &= \\left\\langle \\hbar\\hat{k} \\right\\rangle\\\\\n",
      "&= \\hbar \\left\\langle \\psi(k)\\left|\\hat{k}\\right|\\psi(k) \\right\\rangle\\\\\n",
      "&= \\hbar \\int_{-\\infty}^\\infty\\psi^*(k)k\\psi(k)dk\\\\\n",
      "&= \\hbar \\int_{-\\infty}^\\infty \\frac{1}{\\sqrt{2\\pi}}\\int_{-\\infty}^\\infty \\psi^*(x')e^{-ikx'} k\\frac{1}{\\sqrt{2\\pi}}\\int_{-\\infty}^\\infty \\psi(x)e^{ikx}dxdx'dk\\\\\n",
      "&= \\frac{\\hbar}{2\\pi} \\int_{-\\infty}^\\infty \\psi^*(x')\\int_{-\\infty}^\\infty e^{-ikx'} k\\int_{-\\infty}^\\infty \\psi(x)e^{ikx}dxdkdx'\\\\\n",
      "&= -i\\frac{\\hbar}{2\\pi} \\int_{-\\infty}^\\infty \\psi^*(x')\\int_{-\\infty}^\\infty e^{-ikx'} \\int_{-\\infty}^\\infty \\psi(x)ike^{ikx}dxdkdx'\\\\\n",
      "&= -i\\frac{\\hbar}{2\\pi} \\int_{-\\infty}^\\infty \\psi^*(x')\\int_{-\\infty}^\\infty e^{-ikx'} \\int_{-\\infty}^\\infty \\psi(x)\\frac{d}{dx}e^{ikx}dxdkdx'\\\\\n",
      "\\end{align*}\n",
      "\n",
      "Consider for a moment\n",
      "\n",
      "\\begin{align*}\n",
      "\\int_{-\\infty}^\\infty \\psi(x)\\frac{d}{dx}e^{ikx}dx&=\\psi(x)e^{ikx}\\bigg|_{-\\infty}^\\infty-\\int_{-\\infty}^\\infty \\frac{d}{dx}\\left(\\psi(x)\\right)e^{ikx}dx\\\\\n",
      "\\end{align*}\n",
      "\n",
      "For the square integrable functions $\\psi{x}$ and $e^{ikx}$\n",
      "\n",
      "\\begin{align*}\\psi(x)e^{ikx}\\bigg|_{-\\infty}^\\infty&= 0\n",
      "\\end{align*}\n",
      "\n",
      "\n",
      "\\begin{align*}\n",
      "\\int_{-\\infty}^\\infty \\psi(x)\\frac{d}{dx}e^{ikx}dx&=-\\int_{-\\infty}^\\infty e^{ikx}\\frac{d}{dx}\\psi(x)dx\\\\\n",
      "\\end{align*}\n",
      "\n",
      "Then,\n",
      "\n",
      "\\begin{align*}\n",
      "\\left\\langle \\hat{p}_x \\right\\rangle \n",
      "&= i\\frac{\\hbar}{2\\pi} \\int_{-\\infty}^\\infty \\psi^*(x')\\int_{-\\infty}^\\infty e^{-ikx'} \\int_{-\\infty}^\\infty e^{ikx}\\frac{d}{dx}\\psi(x)dxdkdx'\\\\\n",
      "&= i\\frac{\\hbar}{2\\pi} \\int_{-\\infty}^\\infty \\int_{-\\infty}^\\infty\\int_{-\\infty}^\\infty \\psi^*(x') e^{ik(x-x')}  \\frac{d}{dx}\\psi(x)dxdkdx'\\\\\n",
      "\\end{align*}\n",
      "\n",
      "The Dirac Delta Measure gives \n",
      "\n",
      "\\begin{align*}\n",
      "\\int_{-\\infty}^\\infty e^{ik(x-x')} dk &=2\\pi\\delta(x-x')\n",
      "\\end{align*}\n",
      "\n",
      "So,\n",
      "\n",
      "\\begin{align*}\n",
      "\\left\\langle \\hat{p}_x \\right\\rangle &= -i\\hbar  \\int_{-\\infty}^\\infty\\int_{-\\infty}^\\infty \\psi^*(x') \\delta(x'-x)  \\frac{d}{dx}\\psi(x)dxdx'\\\\\n",
      "&=  \\int_{-\\infty}^\\infty \\psi^*(x) \\left( -i\\hbar  \\frac{d}{dx}\\right)\\psi(x)dx\\\\\n",
      "&= \\left\\langle \\psi^*(x)\\left|\\left( -i\\hbar  \\frac{d}{dx}\\right)\\right|\\psi(x)\\right\\rangle\n",
      "\\end{align*}\n",
      "\n",
      "And therefore, $p_x=-i\\hbar  \\frac{d}{dx}$."
     ]
    },
    {
     "cell_type": "code",
     "collapsed": false,
     "input": [],
     "language": "python",
     "metadata": {},
     "outputs": []
    }
   ],
   "metadata": {}
  }
 ]
}